

HW2 Jacob Manning

1a. Prove the product of two upper triangular matrices are upper triangular.

Let U_1, U_2 be upper triangular. It follows $U_{ij} = 0 = U_{2ij}$ $\forall i > j$. Consider $U_0 = U_1 U_2$. $U_{ij} = \sum_{k=1}^n U_{1ik} U_{2kj}$. Since $U_{1ij} = 0 \forall i > j$, $U_{0ij} = 0 \forall i > j$. $\therefore U_0$ is also upper triangular.

b. Prove the inverse of a nonsingular upper triangular matrix is upper triangular.

Let U be upper triangular and nonsingular. Consider $U^{-1}U = I$. It follows $\delta_{ij} = \sum_{k=1}^n U^{-1}_{ik} U_{kj}$. Since $U_{ij} = 0 \forall i > j$, U^{-1}_{ij} will also need to be zero $\forall i > j$ so that the sum of the products equals δ_{ij} . $\therefore U^{-1}$ is also upper triangular.

2. $A = \begin{bmatrix} 1 & 2 & -1 \\ 1 & 2 & 3 \\ 2 & -1 & 4 \end{bmatrix}$ $b = [-2 \ 10 \ 14]^T$

$[A|b] = \begin{bmatrix} 1 & 2 & -1 & -2 \\ 1 & 2 & 3 & 10 \\ 2 & -1 & 4 & 14 \end{bmatrix}$

$P_{31}[A|b] = \begin{bmatrix} 2 & -1 & 4 & 14 \\ 1 & 2 & 3 & 10 \\ 1 & 2 & -1 & -2 \end{bmatrix}$

$L = \begin{bmatrix} 1 & 0 & 0 \\ \frac{1}{2} & 1 & 0 \\ \frac{1}{2} & 1 & 1 \end{bmatrix}$

$M P_{31}[A|b] = \begin{bmatrix} 2 & -1 & 4 & 14 \\ 0 & \frac{3}{2} & 1 & 3 \\ 0 & \frac{3}{2} & -3 & -9 \end{bmatrix}$

$\hat{M} P_{31}[A|b] = \begin{bmatrix} 2 & -1 & 4 & 14 \\ 0 & \frac{3}{2} & 1 & 3 \\ 0 & 0 & -4 & -12 \end{bmatrix}$

$U = \begin{bmatrix} 2 & -1 & 4 \\ 0 & \frac{3}{2} & 1 \\ 0 & 0 & -4 \end{bmatrix}$

$P_{31}A = LU$

$A = P_{31}LU$

$P_{31}LUx = b$

back sub

$LUx = P_{31}b$

$\begin{bmatrix} 1 & 0 & 0 \\ \frac{1}{2} & 1 & 0 \\ \frac{1}{2} & 1 & 1 \end{bmatrix} Ux = \begin{bmatrix} 14 \\ 10 \\ -2 \end{bmatrix}$

Front sub

$Ux = [14 \ 3 \ -12]^T$

$\begin{bmatrix} 2 & -1 & 4 \\ 0 & \frac{3}{2} & 1 \\ 0 & 0 & -4 \end{bmatrix} x = \begin{bmatrix} 14 \\ 3 \\ -12 \end{bmatrix}$

$x = [1 \ 0 \ 3]^T$

3a. $n \times n$ upper Hessenberg, nonsingular no pivoting

Let A_{in} be the matrix A but with gaussian elimination in $[a_{ij}]$

$A_{i+1:n} = L_i A_{i+1:n}$ $L = \prod_{i=1}^{n-1} L_i$ and $U = A_n = L A = \prod_{i=1}^{n-1} L_i A_0$

b. $L_{ii} = 1 \ 1 \leq i \leq n$ & $L_{i+1,i} = \alpha$ where α is a scalar else $L_{ij} = 0$

c. We would still need $\sim O(n^2)$ operations because we need back substitution

4. This algorithm is numerically stable.
 The stability comes from the fact that all permutations of size $n \times n$ are normal in $\mathbb{R}^{n \times n}$ ($P \in \mathbb{R}^{n \times n}$). You can always find a permutation to commute with any change made to A . It follows permutations are the same done before or after LU factorization. By the numerical stability of $A=LU$, it follows $PA=LU$ is also stable.

5.
$$\begin{bmatrix} L_1 & 0 \\ L_2 & L_2 \end{bmatrix} \begin{bmatrix} x \\ y \end{bmatrix} = \begin{bmatrix} b \\ c \end{bmatrix}$$

First solve $L_1 x = b$ for $x \Rightarrow x = L_1^{-1} b$

Next $Bx + L_2 y = c$ since $x = L_1^{-1} b$ it follows

$$B L_1^{-1} b + L_2 y = c$$

$$L_2 y = c - B L_1^{-1} b$$

Then solve this vector equation for y .

It follows
$$\begin{bmatrix} x \\ y \end{bmatrix} = \begin{bmatrix} L_1^{-1} b \\ L_2^{-1} (c - B L_1^{-1} b) \end{bmatrix}$$